simulations/ctxrefine/CtxRefine.v
@@ -1,31 +1,102 @@
-Require Export Coqlib sflib.
+Require Export Coqlib sflib Any.
 Require Import Behavior.
-Require Import Mod Skeleton.
-  
-Section CTX_REFINE.
-  Context `{Sk.ld}.
-  (* Contexts can be simplified as a single module (by module-linking) *)
-  Definition ctx_refines (md_tgt md_src: Mod.t): Prop :=
-    forall (ctx: Mod.t),
-      Beh.of_program (Mod.compile (Mod.add md_tgt ctx)) <1=
-      Beh.of_program (Mod.compile (Mod.add md_src ctx)).
+Require Import Mod Skeleton ModSimFacts.
+Require Import PCM IPM HMod ISimCore.
+Require Import ModSim.
 
-  Definition refines_closed (md_tgt md_src: Mod.t): Prop :=
+
+Section REFINE.
+  Context `{Sk.ld}.
+
+  Definition refines_mod (md_src md_tgt: Mod.t): Prop :=
     Beh.of_program (Mod.compile md_tgt) <1= Beh.of_program (Mod.compile md_src).
 
-  Definition ctx_refines_list (md_tgt md_src: list Mod.t): Prop :=
-    ctx_refines (Mod.add_list md_tgt) (Mod.add_list md_src).
+End REFINE.
+
+Section CTX_REFINE.
+  (* Definition of ctx refinement in HMod Level. *)
+  Context `{Σ: GRA.t}.
+  Context `{Sk.ld}.
+
+  Definition refines (md_src md_tgt: HMod.t): Prop :=
+    let Ps := HModSem.initial_cond (md_src.(HMod.get_modsem) md_src.(HMod.sk)) in
+    let Pt := HModSem.initial_cond (md_tgt.(HMod.get_modsem) md_tgt.(HMod.sk)) in
+    (* (exists r, Ps r) /\ 
+    (exists r, Pt r) /\ *)
+    (forall rs rt (SRC: Ps rs) (TGT: Pt rt),
+      refines_mod (HMod.to_mod md_src rs) (HMod.to_mod md_tgt rt)).
+
+  Definition ctx_refines (md_src md_tgt: HMod.t): Prop :=
+    forall (ctx: HMod.t),
+      refines (HMod.add md_src ctx) (HMod.add md_tgt ctx).
+
+
+  (* To be moved *)
+  Theorem adequacy_hmod
+      (md_src md_tgt: HMod.t) Ist
+      (rs rt: Σ) 
+      (SIM: HModR.sim md_src md_tgt Ist)
+      (SRC: HModSem.initial_cond (md_src.(HMod.get_modsem) md_src.(HMod.sk)) rs)
+      (TGT: HModSem.initial_cond (md_tgt.(HMod.get_modsem) md_tgt.(HMod.sk)) rt)
+    :
+      ModR.sim (HMod.to_mod md_src rs) (HMod.to_mod md_tgt rt).
+  Proof.
+  Admitted.
+
+    Theorem isim_ctx
+            ctx ms1 ms2 Ist
+            (SIM: HModSemR.sim ms1 ms2 Ist)
+        :
+            HModSemR.sim (HModSem.add ms1 ctx) (HModSem.add ms2 ctx) (IstProd Ist IstEq).
+    Proof.
+    Admitted.
+  
+  Lemma hmod_sim_refl md:
+       HModSemR.sim md md IstEq. 
+  Proof. Admitted.
 
 End CTX_REFINE.
 
 Section PROPERTIES.
   Context `{Sk.ld}.
 
-  (*** vertical composition ***)
-  Global Program Instance refines_PreOrder: PreOrder ctx_refines.
-
+  (*** refines_mod ***)
+  Global Program Instance refines_mod_PreOrder: PreOrder refines_mod.
   Next Obligation. ii. ss. Qed.
-  Next Obligation. ii. eapply H1. eapply H0. ss. Qed.
+  Next Obligation. ii. eapply H0. eapply H1. ss. Qed.
+
+  Context `{Σ: GRA.t}.
+
+  Global Program Instance refines_PreOrder: PreOrder refines.
+  Next Obligation. Admitted.
+    (* do 2 r. i.   
+      eapply adequacy_mod, adequacy_hmod; ss. 
+      econs; ss. i. eapply hmod_sim_refl.
+  
+  Qed. *)
+  Next Obligation.
+    ii. rr in H0. rr in H1. des.
+    rr. esplits. 
+    { eauto. }
+    { eauto. }
+    i.
+    specialize (H5 rs r2 SRC H4).
+    specialize (H3 r2 rt H4 TGT).
+    r. i. eapply H5. eapply H3. eauto.
+  Admitted.
+
+
+  (*** vertical composition ***)
+  Global Program Instance ctx_refines_PreOrder: PreOrder ctx_refines.
+
+  Next Obligation. 
+    do 3 r. i. eapply adequacy_mod. eapply adequacy_hmod; eauto.
+    instantiate (1:= IstProd IstEq IstEq).
+    econs; eauto. i. rr. eapply isim_ctx, hmod_sim_refl. 
+  Qed.
+  Next Obligation. do 2 r. i. 
+  
+  eapply H1. eapply H0. ss. Qed.
 
   Global Program Instance refines2_PreOrder: PreOrder ctx_refines_list.
   Next Obligation.
